## Model

### Original

$
\text{predecessor\_util}(l_1l_2...l_n)  = \begin{cases}
([], 1) &\text{if } n = 0\\
((l_1 - 1) \oplus list, 0) &\text{if } flag = 1 \land l_1 \neq 0,\text{where } (list, flag) = predecessor\_util(l_2...l_n)\\ 
(9 \oplus list , 1) &\text{if } flag = 1 \land l_1 = 0,\text{where } (list, flag) = predecessor\_util(l_2...l_n)\\ 
(l_1 \oplus list, 0) &\text{otherwise},\text{where } (list, flag) = predecessor\_util(l_2...l_n)\\ 
\end{cases}
$

### Refactored:

$
\text{predecessor\_util}(l_1l_2...l_n)  = \begin{cases}
([], 1) &\text{if } n = 0\\
(d \oplus list, f) &\text{otherwise } {where } (list, flag) = predecessor\_util(l_2...l_n)\\
&  \text{and } (d,f)=aux(l_1,flag)\\ 
\end{cases}
$
$aux(d,f)= \begin{cases}
(d,f),&\text{if } f = 0\\
(9,1),&\text{if } f = 1 \land d = 0\\
(d-1,0),&\text{if } f = 1 \land d \neq 0\\
\end{cases}
$

---

$
\text{remove\_redunandant}(l_1l_2...l_n)=\begin{cases}
l_2...l_n, &\text{if } n >= 2 \land l_1 \neq 0\\
l_1...l_n, &\text{otherwise}
\end{cases}
$


$
\text{predecessor}(l)=\text{remove\_redundant}(list),\text{where (list, \_)=\text{predecessor\_util}(l)}
$

$\text{predecessor\_list}(l_1l_2...l_n)= \begin{cases}
[] &\text{if } n = 0\\
\text{predecessor}(l_1) \oplus \text{predecessor\_list}(l_2...l_n),& \text{if } n > 0 \land l_1 \text{is a list}\\ 
l_1 \oplus \text{predecessor\_list}(l_2...l_n),& \text{otherwise }\\ 
\end{cases}
$